src/cbor/pulse/raw/CBOR.Pulse.Raw.Format.Serialize.fsti
@@ -1,1 +1,23 @@
 module CBOR.Pulse.Raw.Format.Serialize
+include CBOR.Pulse.Raw.Match
+open CBOR.Spec.Raw.Format
+open Pulse.Lib.Pervasives
+open Pulse.Lib.Trade
+
+module U8 = FStar.UInt8
+module SZ = FStar.SizeT
+module Trade = Pulse.Lib.Trade.Util
+module S = Pulse.Lib.Slice
+
+val cbor_serialize
+  (x: cbor_raw)
+  (output: S.slice U8.t)
+  (#y: Ghost.erased raw_data_item)
+  (#pm: perm)
+: stt SZ.t
+    (exists* v . cbor_match pm x y ** S.pts_to output v ** pure (Seq.length (serialize_cbor y) <= SZ.v (S.len output)))
+    (fun res -> exists* v . cbor_match pm x y ** S.pts_to output v ** pure (
+      let s = serialize_cbor y in
+      SZ.v res == Seq.length s /\
+      (exists v' . v `Seq.equal` (s `Seq.append` v'))
+    ))
